num/W.v
@@ -3,7 +3,7 @@ Set Implicit Arguments.
 Require Import Basic_type.
 Require Import ZnZ.
 Require Import Zn2Z.
-Require Import W2_op.
+Require Import W8_op.
 Require Import ZArith.
 Require Import MkSpec.
 
@@ -15,7 +15,7 @@ Require Import MkSpec.
 Definition mk_word (w: Set) (n:nat): Set.
 fix 2.
 intros w n; case n; simpl.
-exact w2.
+exact w8.
 intros n1; exact (zn2z (mk_word w n1)).
 Defined.
 
@@ -48,105 +48,105 @@ rewrite Zpower_exp; auto with zarith.
 Qed.
 
 (* ** Operators ** *)
-Definition w2_1_op := mk_zn2z_op w2_op.           
-Definition w2_2_op := mk_zn2z_op w2_1_op.
-Definition w2_3_op := mk_zn2z_op w2_2_op.
-Definition w2_4_op := mk_zn2z_op_karatsuba w2_3_op.
-Definition w2_5_op := mk_zn2z_op_karatsuba w2_4_op.
-Definition w2_6_op := mk_zn2z_op_karatsuba w2_5_op.
-Definition w2_7_op := mk_zn2z_op_karatsuba w2_6_op.
-Definition w2_8_op := mk_zn2z_op_karatsuba w2_7_op.
-Definition w2_9_op := mk_zn2z_op_karatsuba w2_8_op.
-Definition w2_10_op := mk_zn2z_op_karatsuba w2_9_op.
-Definition w2_11_op := mk_zn2z_op_karatsuba w2_10_op.
-Definition w2_12_op := mk_zn2z_op_karatsuba w2_11_op.
-Definition w2_13_op := mk_zn2z_op_karatsuba w2_12_op.
-Definition w2_14_op := mk_zn2z_op_karatsuba w2_13_op.
+Definition w8_1_op := mk_zn2z_op w8_op.           
+Definition w8_2_op := mk_zn2z_op w8_1_op.
+Definition w8_3_op := mk_zn2z_op w8_2_op.
+Definition w8_4_op := mk_zn2z_op_karatsuba w8_3_op.
+Definition w8_5_op := mk_zn2z_op_karatsuba w8_4_op.
+Definition w8_6_op := mk_zn2z_op_karatsuba w8_5_op.
+Definition w8_7_op := mk_zn2z_op_karatsuba w8_6_op.
+Definition w8_8_op := mk_zn2z_op_karatsuba w8_7_op.
+Definition w8_9_op := mk_zn2z_op_karatsuba w8_8_op.
+Definition w8_10_op := mk_zn2z_op_karatsuba w8_9_op.
+Definition w8_11_op := mk_zn2z_op_karatsuba w8_10_op.
+Definition w8_12_op := mk_zn2z_op_karatsuba w8_11_op.
+Definition w8_13_op := mk_zn2z_op_karatsuba w8_12_op.
+Definition w8_14_op := mk_zn2z_op_karatsuba w8_13_op.
 
-Definition cmk_op (n: nat): znz_op (word w2 n).
+Definition cmk_op (n: nat): znz_op (word w8 n).
 intros n; case n; clear n.
-exact w2_op.
+exact w8_op.
 intros n; case n; clear n.
-exact w2_1_op.
+exact w8_1_op.
 intros n; case n; clear n.
-exact w2_2_op.
+exact w8_2_op.
 intros n; case n; clear n.
-exact w2_3_op.
+exact w8_3_op.
 intros n; case n; clear n.
-exact w2_4_op.
+exact w8_4_op.
 intros n; case n; clear n.
-exact w2_5_op.
+exact w8_5_op.
 intros n; case n; clear n.
-exact w2_6_op.
+exact w8_6_op.
 intros n; case n; clear n.
-exact w2_7_op.
+exact w8_7_op.
 intros n; case n; clear n.
-exact w2_8_op.
+exact w8_8_op.
 intros n; case n; clear n.
-exact w2_9_op.
+exact w8_9_op.
 intros n; case n; clear n.
-exact w2_10_op.
+exact w8_10_op.
 intros n; case n; clear n.
-exact w2_11_op.
+exact w8_11_op.
 intros n; case n; clear n.
-exact w2_12_op.
+exact w8_12_op.
 intros n; case n; clear n.
-exact w2_13_op.
+exact w8_13_op.
 intros n; case n; clear n.
-exact w2_14_op.
+exact w8_14_op.
 intros n.
 match goal with |- context[S ?X] =>
- exact (mk_op w2_op (S X))
+ exact (mk_op w8_op (S X))
 end.
 Defined.
 
-Require Import W2_op_spec.
+Require Import W8_op_spec.
 
 Definition cmk_spec n: znz_spec (cmk_op n).
-assert (S1: znz_spec w2_1_op).
-unfold w2_1_op; apply mk_znz2_spec.
-exact w2_op_spec.
-assert (S2: znz_spec w2_2_op).
-unfold w2_2_op; apply mk_znz2_spec.
+assert (S1: znz_spec w8_1_op).
+unfold w8_1_op; apply mk_znz2_spec.
+exact w8_op_spec.
+assert (S2: znz_spec w8_2_op).
+unfold w8_2_op; apply mk_znz2_spec.
 exact S1.
-assert (S3: znz_spec w2_3_op).
-unfold w2_3_op; apply mk_znz2_spec.
+assert (S3: znz_spec w8_3_op).
+unfold w8_3_op; apply mk_znz2_spec.
 exact S2.
-assert (S4: znz_spec w2_4_op).
-unfold w2_4_op; apply mk_znz2_karatsuba_spec.
+assert (S4: znz_spec w8_4_op).
+unfold w8_4_op; apply mk_znz2_karatsuba_spec.
 exact S3.
-assert (S5: znz_spec w2_5_op).
-unfold w2_5_op; apply mk_znz2_karatsuba_spec.
+assert (S5: znz_spec w8_5_op).
+unfold w8_5_op; apply mk_znz2_karatsuba_spec.
 exact S4.
-assert (S6: znz_spec w2_6_op).
-unfold w2_6_op; apply mk_znz2_karatsuba_spec.
+assert (S6: znz_spec w8_6_op).
+unfold w8_6_op; apply mk_znz2_karatsuba_spec.
 exact S5.
-assert (S7: znz_spec w2_7_op).
-unfold w2_7_op; apply mk_znz2_karatsuba_spec.
+assert (S7: znz_spec w8_7_op).
+unfold w8_7_op; apply mk_znz2_karatsuba_spec.
 exact S6.
-assert (S8: znz_spec w2_8_op).
-unfold w2_8_op; apply mk_znz2_karatsuba_spec.
+assert (S8: znz_spec w8_8_op).
+unfold w8_8_op; apply mk_znz2_karatsuba_spec.
 exact S7.
-assert (S9: znz_spec w2_9_op).
-unfold w2_9_op; apply mk_znz2_karatsuba_spec.
+assert (S9: znz_spec w8_9_op).
+unfold w8_9_op; apply mk_znz2_karatsuba_spec.
 exact S8.
-assert (S10: znz_spec w2_10_op).
-unfold w2_10_op; apply mk_znz2_karatsuba_spec.
+assert (S10: znz_spec w8_10_op).
+unfold w8_10_op; apply mk_znz2_karatsuba_spec.
 exact S9.
-assert (S11: znz_spec w2_11_op).
-unfold w2_11_op; apply mk_znz2_karatsuba_spec.
+assert (S11: znz_spec w8_11_op).
+unfold w8_11_op; apply mk_znz2_karatsuba_spec.
 exact S10.
-assert (S12: znz_spec w2_12_op).
-unfold w2_12_op; apply mk_znz2_karatsuba_spec.
+assert (S12: znz_spec w8_12_op).
+unfold w8_12_op; apply mk_znz2_karatsuba_spec.
 exact S11.
-assert (S13: znz_spec w2_13_op).
-unfold w2_13_op; apply mk_znz2_karatsuba_spec.
+assert (S13: znz_spec w8_13_op).
+unfold w8_13_op; apply mk_znz2_karatsuba_spec.
 exact S12.
-assert (S14: znz_spec w2_14_op).
-unfold w2_14_op; apply mk_znz2_karatsuba_spec.
+assert (S14: znz_spec w8_14_op).
+unfold w8_14_op; apply mk_znz2_karatsuba_spec.
 exact S13.
 intros n; case n; clear n.
-exact w2_op_spec.
+exact w8_op_spec.
 intros n; case n; clear n.
 exact S1.
 intros n; case n; clear n.
@@ -182,13 +182,13 @@ repeat match goal with |- znz_spec (mk_zn2z_op_karatsuba ?X) =>
   apply tmp; clear tmp
 end.
 apply mk_spec.
-exact w2_op_spec.
+exact w8_op_spec.
 Defined.
 
 
 Theorem cmk_op_digits: forall n, 
-  (Zpos (znz_digits (cmk_op n)) = 2 ^ (Z_of_nat n + 1))%Z.
-do 15 (intros n; case n; clear n; [reflexivity | idtac]).
+  (Zpos (znz_digits (cmk_op n)) = 2 ^ (Z_of_nat n + 3))%Z.
+do 15 (intros n; case n; clear n; [try reflexivity | idtac]).
 intros n; unfold cmk_op; lazy beta.
 rewrite mk_op_digits; auto.
 rewrite Zpower_exp; auto with zarith.
